compress_extra

Primitive_Matchers/Transform.thy
@@ -6,6 +6,40 @@ imports "Common_Primitive_Matcher"
         "../Primitive_Matchers/IpAddresses_Normalize"
 begin
 
+
+
+(*TODO: move
+  TODO: this is currently not used.*)
+text{*Compress many @{const Extra} expressions to one expression.*}
+fun compress_extra :: "common_primitive match_expr \<Rightarrow> common_primitive match_expr" where
+  "compress_extra (Match x) = Match x" |
+  "compress_extra (MatchNot (Match (Extra e))) = Match (Extra (''NOT ''@e))" |
+  "compress_extra (MatchNot m) = (MatchNot (compress_extra m))" |
+  "compress_extra (MatchAnd (Match (Extra e1)) (Match (Extra e2))) = compress_extra (Match (Extra (e1@'' ''@e2)))" |
+  "compress_extra (MatchAnd m1 m2) = (case (compress_extra m1, compress_extra m2) of 
+        (Match (Extra e1), Match (Extra e2)) \<Rightarrow> Match (Extra (e1@'' ''@e2))
+      | (m1', m2') \<Rightarrow> MatchAnd m1' m2')" |
+  "compress_extra MatchAny = MatchAny"
+
+value "compress_extra (MatchAnd (Match (Extra ''foo'')) (MatchNot (Match (Extra ''bar''))))"
+value "compress_extra (MatchAnd (Match (Extra ''foo'')) (Match (Extra ''bar'')))"
+
+lemma compress_extra_correct_matchexpr: "matches (common_matcher, \<alpha>) m = matches (common_matcher, \<alpha>) (compress_extra m)"
+  proof(simp add: fun_eq_iff, clarify, rename_tac a p)
+    fix a p
+    have "ternary_ternary_eval (map_match_tac common_matcher p m) = ternary_ternary_eval (map_match_tac common_matcher p (compress_extra m))"
+      apply(induction m rule: compress_extra.induct)
+      apply (simp_all)
+      apply(simp_all add: eval_ternary_simps)
+      apply(simp_all split: match_expr.split match_expr.split_asm common_primitive.split)
+      apply(simp add: eval_ternary_simps_simple)
+      done (*TODO: tune proof*)
+    thus "matches (common_matcher, \<alpha>) m a p = matches (common_matcher, \<alpha>) (compress_extra m) a p"
+      by(rule matches_iff_apply_f)
+    qed
+
+
+
 (*closure bounds*)
 
 (*def: transform_optimize = optimize_matches opt_MatchAny_match_expr \<circ> optimize_matches optimize_primitive_univ
